tests/compiler/foreign/main.lean
@@ -3,13 +3,13 @@ constant SPointed : PointedType
 def S : Type := SPointed.type
 instance : Inhabited S := ⟨SPointed.val⟩
 
-@[extern "lean_mk_S"] constant mkS (x y : UInt32) (s : @& String) : S := arbitrary _
-@[extern "lean_S_add_x_y"] constant S.addXY (s : @& S) : UInt32 := arbitrary _
-@[extern "lean_S_string"] constant S.string (s : @& S) : String := arbitrary _
+@[extern "lean_mk_S"] constant mkS (x y : UInt32) (s : @& String) : S
+@[extern "lean_S_add_x_y"] constant S.addXY (s : @& S) : UInt32
+@[extern "lean_S_string"] constant S.string (s : @& S) : String
 -- The following 3 externs have side effects. Thus, we put them in IO.
-@[extern "lean_S_global_append"] constant appendToGlobalS (str : @& String) : IO Unit := arbitrary _
-@[extern "lean_S_global_string"] constant getGlobalString : IO String := arbitrary _
-@[extern "lean_S_update_global"] constant updateGlobalS (s : @& S) : IO Unit := arbitrary _
+@[extern "lean_S_global_append"] constant appendToGlobalS (str : @& String) : IO Unit
+@[extern "lean_S_global_string"] constant getGlobalString : IO String
+@[extern "lean_S_update_global"] constant updateGlobalS (s : @& S) : IO Unit
 
 def main : IO Unit := do
 IO.println (mkS 10 20 "hello").addXY;
