tests/lean/run/optParam.lean
@@ -8,10 +8,10 @@ theorem ex2 : p (x := 1) |>.2 = 1 :=
 rfl
 
 def c {α : Type} [Inhabited α] : α × α :=
-(arbitrary _, arbitrary _)
+(arbitrary, arbitrary)
 
-theorem ex3 {α} [Inhabited α] : c.1 = arbitrary α :=
+theorem ex3 {α} [Inhabited α] : c.1 = arbitrary (α := α) :=
 rfl
 
-theorem ex4 {α} [Inhabited α] : c.2 = arbitrary α :=
+theorem ex4 {α} [Inhabited α] : c.2 = arbitrary (α := α) :=
 rfl
